Complete generalized term rewriting

ffi/ByteStringFFI.v
@@ -5,6 +5,7 @@ Require Import
   ByteString.Lib.TupleEnsembles
   ByteString.Lib.FunMaps
   ByteString.Lib.FromADT
+  ByteString.Lib.HList
   ByteString.Memory
   ByteString.Heap
   ByteString.FFI.HeapFFI
@@ -17,41 +18,11 @@ Require Import
   Hask.Control.Monad.Trans.FiatState
   Hask.Control.Monad.Free.
 
-Inductive hlist : list Type -> Type :=
-  | HNil : hlist []
-  | HCons : forall t ts, t -> hlist ts -> hlist (t :: ts).
+(****************************************************************************
+ * ClientDSL: DSL that represents a series of calls against an ADT signature
+ ****************************************************************************)
 
-Import EqNotations.
-
-Lemma cons_head_eq : forall A (x0 : A) x1 y0 y1,
-  x0 :: y0 = x1 :: y1 -> x0 = x1.
-Proof.
-  intros.
-  inv H.
-  intuition.
-Defined.
-
-Lemma cons_tail_eq : forall A (x0 : A) x1 y0 y1,
-  x0 :: y0 = x1 :: y1 -> y0 = y1.
-Proof.
-  intros.
-  inv H.
-  intuition.
-Defined.
-
-Program Definition hlist_head `(l : hlist (t :: ts)) : t :=
-  match l in hlist d return d = t :: ts -> t with
-  | HNil => fun _ => False_rect _ _
-  | HCons _ _ x _ => fun H => rew (cons_head_eq H) in x
-  end eq_refl.
-
-Program Definition hlist_tail `(l : hlist (t :: ts)) : hlist ts :=
-  match l in hlist d return d = t :: ts -> hlist ts with
-  | HNil => fun _ => False_rect _ _
-  | HCons _ _ _ xs => fun H => rew (cons_tail_eq H) in xs
-  end eq_refl.
-
-Section Reflection.
+Section ClientDSL.
 
 Variable sig : ADTSig.
 
@@ -68,11 +39,14 @@ Global Program Instance MethodCall_Functor : Functor MethodCall := {
     end
 }.
 
-Definition CallDSL := Free MethodCall.
+Definition ClientDSL := Free MethodCall.
+
+(****************************************************************************
+ * ADT_Computes: Relates a [ClientDSL] term to a Fiat computation using an
+ * ADT of the same signature.
+ ****************************************************************************)
 
 Variable adt : ADT sig.
-
-Import EqNotations.
 
 Program Fixpoint applyArgs
          (dom : list Type)
@@ -87,6 +61,8 @@ Program Fixpoint applyArgs
       applyArgs (fun r => meth r (hlist_head args))
                 (hlist_tail args)
   end args meth.
+
+Import EqNotations.
 
 Inductive MethodCall_Computes :
   forall A, MethodCall A -> Rep adt -> Rep adt -> A -> Prop :=
@@ -160,19 +136,16 @@ Inductive Free_Computes `{Functor f} {R : Type}
 
 Definition ADT_Computes {A : Type} := Free_Computes (A:=A) MethodCall_Computes.
 
+(****************************************************************************
+ * reflect_ADT_DSL_computation: Helper lemmas to abstract a Fiat
+ * computation into its equivalent [ClientDSL] term.
+ ****************************************************************************)
+
 Definition reflect_ADT_DSL_computation {A B : Type}
            (c : Rep adt * B -> Comp ((Rep adt * B) * A)) :=
-  { f : B -> CallDSL (B * A)
+  { f : B -> ClientDSL (B * A)
   & forall r bs r' bs' v, c (r, bs) ↝ ((r', bs'), v)
       -> ADT_Computes (f bs) r r' (bs', v) }.
-
-Lemma reflect_computation_ret {A B : Type} (v : A) :
-  reflect_ADT_DSL_computation (B:=B) (fun r => ret (r, v)).
-Proof.
-  exists (fun r => pure (r, v)); intros.
-  computes_to_inv; injections.
-  eapply CPure.
-Defined.
 
 Lemma reflect_ADT_DSL_computation_simplify {B C : Type} c c'
       (refine_c_c' : forall r, refineEquiv (c r) (c' r))
@@ -213,31 +186,202 @@ Proof.
   apply a; assumption.
 Defined.
 
-End Reflection.
+End ClientDSL.
 
-Module ByteStringFFI (M : WSfun N_as_DT).
+Arguments MethodCall {sig} rec.
+Arguments Call {sig rec} midx {dom cod} _ _ _ _.
 
-Module Import ByteStringHeap := ByteStringHeap M.
-Module Import FunMaps := FunMaps N_as_DT M.
+(****************************************************************************
+ * [reflect_ADT_DSL_computation] compilation tactics
+ ****************************************************************************)
 
-Import HeapCanonical.
-Import Heap.
-Import HeapState.
-Import FMapExt.
+Ltac wrapup :=
+  first
+  [ eassumption
+  | higher_order_reflexivity
+  | instantiate (1 := eq_sym eq_refl);
+    instantiate (1 := eq_sym eq_refl);
+    reflexivity ].
 
-Definition ByteString (r : Rep HeapSpec) := Rep (projT1 (ByteStringHeap r)).
+Ltac solve_for1 :=
+  match goal with
+  | [ H : _ _ ?A ↝ (?R, _) |- MethodCall_Computes _ _ _ ?R _ ] =>
+    solve [ eapply CallCompute1
+              with (midx := Fin.F1); wrapup ]
+  | [ H : _ _ ?A ↝ (?R, _) |- MethodCall_Computes _ _ _ ?R _ ] =>
+    solve [ eapply CallCompute1
+              with (midx := Fin.FS Fin.F1); wrapup ]
+  | [ H : _ _ ?A ↝ (?R, _) |- MethodCall_Computes _ _ _ ?R _ ] =>
+    solve [ eapply CallCompute1
+              with (midx := Fin.FS (Fin.FS Fin.F1)); wrapup ]
+  | [ H : _ _ ?A ↝ (?R, _) |- MethodCall_Computes _ _ _ ?R _ ] =>
+    solve [ eapply CallCompute1
+              with (midx := Fin.FS (Fin.FS (Fin.FS Fin.F1))); wrapup ]
+  | [ H : _ _ ?A ↝ (?R, _) |- MethodCall_Computes _ _ _ ?R _ ] =>
+    solve [ eapply CallCompute1
+              with (midx := Fin.FS (Fin.FS (Fin.FS (Fin.FS Fin.F1)))); wrapup ]
+  | [ H : _ _ ?A ↝ (?R, _) |- MethodCall_Computes _ _ _ ?R _ ] =>
+    solve [ eapply CallCompute1
+              with (midx := Fin.FS (Fin.FS (Fin.FS (Fin.FS (Fin.FS Fin.F1))))); wrapup ]
+  | [ H : _ _ ?A ↝ (?R, _) |- MethodCall_Computes _ _ _ ?R _ ] =>
+    solve [ eapply CallCompute1
+              with (midx := Fin.FS (Fin.FS (Fin.FS (Fin.FS (Fin.FS (Fin.FS Fin.F1))))));
+                wrapup ]
+  | [ H : _ _ ?A ↝ (?R, _) |- MethodCall_Computes _ _ _ ?R _ ] =>
+    solve [
+      eapply CallCompute1
+        with (midx := Fin.FS (Fin.FS (Fin.FS (Fin.FS (Fin.FS (Fin.FS (Fin.FS Fin.F1)))))));
+          wrapup ]
+  | [ H : _ _ ?A ↝ (?R, _) |- MethodCall_Computes _ _ _ ?R _ ] =>
+    solve [
+      eapply CallCompute1
+        with (midx :=
+                Fin.FS (Fin.FS (Fin.FS (Fin.FS (Fin.FS (Fin.FS (Fin.FS (Fin.FS Fin.F1))))))));
+          wrapup ]
+  end.
 
-Hint Unfold id.
-Hint Unfold bind.
-Hint Unfold Bind2.
-Hint Unfold allocate_buffer.
-Hint Unfold find_free_block.
-Hint Unfold make_room_by_growing_buffer.
-Hint Unfold make_room_by_shifting_up.
-Hint Unfold ByteStringHeap.buffer_cons_obligation_2.
-Hint Unfold ByteStringHeap.buffer_cons_obligation_3.
-Hint Unfold poke_at_offset.
-Hint Unfold buffer_cons.
+Ltac solve_for2 :=
+  match goal with
+  | [ H : _ _ ?A ?B ↝ (?R, _) |- MethodCall_Computes _ _ _ ?R _ ] =>
+    solve [ eapply CallCompute2
+              with (midx := Fin.F1); wrapup ]
+  | [ H : _ _ ?A ?B ↝ (?R, _) |- MethodCall_Computes _ _ _ ?R _ ] =>
+    solve [ eapply CallCompute2
+              with (midx := Fin.FS Fin.F1); wrapup ]
+  | [ H : _ _ ?A ?B ↝ (?R, _) |- MethodCall_Computes _ _ _ ?R _ ] =>
+    solve [ eapply CallCompute2
+              with (midx := Fin.FS (Fin.FS Fin.F1)); wrapup ]
+  | [ H : _ _ ?A ?B ↝ (?R, _) |- MethodCall_Computes _ _ _ ?R _ ] =>
+    solve [ eapply CallCompute2
+              with (midx := Fin.FS (Fin.FS (Fin.FS Fin.F1))); wrapup ]
+  | [ H : _ _ ?A ?B ↝ (?R, _) |- MethodCall_Computes _ _ _ ?R _ ] =>
+    solve [ eapply CallCompute2
+              with (midx := Fin.FS (Fin.FS (Fin.FS (Fin.FS Fin.F1)))); wrapup ]
+  | [ H : _ _ ?A ?B ↝ (?R, _) |- MethodCall_Computes _ _ _ ?R _ ] =>
+    solve [ eapply CallCompute2
+              with (midx := Fin.FS (Fin.FS (Fin.FS (Fin.FS (Fin.FS Fin.F1))))); wrapup ]
+  | [ H : _ _ ?A ?B ↝ (?R, _) |- MethodCall_Computes _ _ _ ?R _ ] =>
+    solve [ eapply CallCompute2
+              with (midx := Fin.FS (Fin.FS (Fin.FS (Fin.FS (Fin.FS (Fin.FS Fin.F1))))));
+                wrapup ]
+  | [ H : _ _ ?A ?B ↝ (?R, _) |- MethodCall_Computes _ _ _ ?R _ ] =>
+    solve [
+      eapply CallCompute2
+        with (midx := Fin.FS (Fin.FS (Fin.FS (Fin.FS (Fin.FS (Fin.FS (Fin.FS Fin.F1)))))));
+          wrapup ]
+  | [ H : _ _ ?A ?B ↝ (?R, _) |- MethodCall_Computes _ _ _ ?R _ ] =>
+    solve [
+      eapply CallCompute2
+        with (midx :=
+                Fin.FS (Fin.FS (Fin.FS (Fin.FS (Fin.FS (Fin.FS (Fin.FS (Fin.FS Fin.F1))))))));
+          wrapup ]
+  end.
+
+Ltac solve_for3 :=
+  match goal with
+  | [ H : _ _ ?A ?B ?C ↝ (?R, _) |- MethodCall_Computes _ _ _ ?R _ ] =>
+    solve [ eapply CallCompute3
+              with (midx := Fin.F1); wrapup ]
+  | [ H : _ _ ?A ?B ?C ↝ (?R, _) |- MethodCall_Computes _ _ _ ?R _ ] =>
+    solve [ eapply CallCompute3
+              with (midx := Fin.FS Fin.F1); wrapup ]
+  | [ H : _ _ ?A ?B ?C ↝ (?R, _) |- MethodCall_Computes _ _ _ ?R _ ] =>
+    solve [ eapply CallCompute3
+              with (midx := Fin.FS (Fin.FS Fin.F1)); wrapup ]
+  | [ H : _ _ ?A ?B ?C ↝ (?R, _) |- MethodCall_Computes _ _ _ ?R _ ] =>
+    solve [ eapply CallCompute3
+              with (midx := Fin.FS (Fin.FS (Fin.FS Fin.F1))); wrapup ]
+  | [ H : _ _ ?A ?B ?C ↝ (?R, _) |- MethodCall_Computes _ _ _ ?R _ ] =>
+    solve [ eapply CallCompute3
+              with (midx := Fin.FS (Fin.FS (Fin.FS (Fin.FS Fin.F1)))); wrapup ]
+  | [ H : _ _ ?A ?B ?C ↝ (?R, _) |- MethodCall_Computes _ _ _ ?R _ ] =>
+    solve [ eapply CallCompute3
+              with (midx := Fin.FS (Fin.FS (Fin.FS (Fin.FS (Fin.FS Fin.F1))))); wrapup ]
+  | [ H : _ _ ?A ?B ?C ↝ (?R, _) |- MethodCall_Computes _ _ _ ?R _ ] =>
+    solve [ eapply CallCompute3
+              with (midx := Fin.FS (Fin.FS (Fin.FS (Fin.FS (Fin.FS (Fin.FS Fin.F1))))));
+                wrapup ]
+  | [ H : _ _ ?A ?B ?C ↝ (?R, _) |- MethodCall_Computes _ _ _ ?R _ ] =>
+    solve [
+      eapply CallCompute3
+        with (midx := Fin.FS (Fin.FS (Fin.FS (Fin.FS (Fin.FS (Fin.FS (Fin.FS Fin.F1)))))));
+          wrapup ]
+  | [ H : _ _ ?A ?B ?C ↝ (?R, _) |- MethodCall_Computes _ _ _ ?R _ ] =>
+    solve [
+      eapply CallCompute3
+        with (midx :=
+                Fin.FS (Fin.FS (Fin.FS (Fin.FS (Fin.FS (Fin.FS (Fin.FS (Fin.FS Fin.F1))))))));
+          wrapup ]
+  end.
+
+Ltac solve_for4 :=
+  match goal with
+  | [ H : _ _ ?A ?B ?C ?D ↝ (?R, _) |- MethodCall_Computes _ _ _ ?R _ ] =>
+    solve [ eapply CallCompute4
+              with (midx := Fin.F1); wrapup ]
+  | [ H : _ _ ?A ?B ?C ?D ↝ (?R, _) |- MethodCall_Computes _ _ _ ?R _ ] =>
+    solve [ eapply CallCompute4
+              with (midx := Fin.FS Fin.F1); wrapup ]
+  | [ H : _ _ ?A ?B ?C ?D ↝ (?R, _) |- MethodCall_Computes _ _ _ ?R _ ] =>
+    solve [ eapply CallCompute4
+              with (midx := Fin.FS (Fin.FS Fin.F1)); wrapup ]
+  | [ H : _ _ ?A ?B ?C ?D ↝ (?R, _) |- MethodCall_Computes _ _ _ ?R _ ] =>
+    solve [ eapply CallCompute4
+              with (midx := Fin.FS (Fin.FS (Fin.FS Fin.F1))); wrapup ]
+  | [ H : _ _ ?A ?B ?C ?D ↝ (?R, _) |- MethodCall_Computes _ _ _ ?R _ ] =>
+    solve [ eapply CallCompute4
+              with (midx := Fin.FS (Fin.FS (Fin.FS (Fin.FS Fin.F1)))); wrapup ]
+  | [ H : _ _ ?A ?B ?C ?D ↝ (?R, _) |- MethodCall_Computes _ _ _ ?R _ ] =>
+    solve [ eapply CallCompute4
+              with (midx := Fin.FS (Fin.FS (Fin.FS (Fin.FS (Fin.FS Fin.F1))))); wrapup ]
+  | [ H : _ _ ?A ?B ?C ?D ↝ (?R, _) |- MethodCall_Computes _ _ _ ?R _ ] =>
+    solve [ eapply CallCompute4
+              with (midx := Fin.FS (Fin.FS (Fin.FS (Fin.FS (Fin.FS (Fin.FS Fin.F1))))));
+                wrapup ]
+  | [ H : _ _ ?A ?B ?C ?D ↝ (?R, _) |- MethodCall_Computes _ _ _ ?R _ ] =>
+    solve [
+      eapply CallCompute4
+        with (midx := Fin.FS (Fin.FS (Fin.FS (Fin.FS (Fin.FS (Fin.FS (Fin.FS Fin.F1)))))));
+          wrapup ]
+  | [ H : _ _ ?A ?B ?C ?D ↝ (?R, _) |- MethodCall_Computes _ _ _ ?R _ ] =>
+    solve [
+      eapply CallCompute4
+        with (midx :=
+                Fin.FS (Fin.FS (Fin.FS (Fin.FS (Fin.FS (Fin.FS (Fin.FS (Fin.FS Fin.F1))))))));
+          wrapup ]
+  end.
+
+Ltac solve_for_call :=
+  first [ solve_for1 | solve_for2 | solve_for3 | solve_for4 ].
+
+Ltac tsubst :=
+  repeat
+    match goal with
+    | [ H : (_, _) = (_, _) |- _ ] => inv H
+    | [ H : (_, _, _) = (_, _, _) |- _ ] => inv H
+    | [ H : (_, _, _, _) = (_, _, _, _) |- _ ] => inv H
+    end;
+  subst.
+
+Ltac build_computational_spine :=
+  repeat match goal with
+  | [ |- reflect_ADT_DSL_computation _ _ ] => eexists; intros
+  | H : {a' | @?P a'} ↝ _ |- _ => apply Pick_inv in H
+  | H : Return ?a ↝ _ |- _ =>
+    apply Return_inv in H; tsubst; try apply CPure
+  | H : Bind (A := ?A) ?ca ?k ↝ _ |- _ =>
+    apply Bind_inv in H;
+    let a' := fresh "v" in
+    let H' := fresh H "'" in
+    destruct H as [a' [H H'] ];
+    eapply CJoin
+  end;
+  computes_to_inv; tsubst; simpl in *;
+  repeat match goal with
+  | [ H : _ * _ |- _ ] => destruct H
+  | [ H : () |- _ ] => destruct H
+  end;
+  first [ solve_for_call | simpl in *; solve_for_call ].
 
 Ltac simplify_reflection :=
   eapply reflect_ADT_DSL_computation_simplify;
@@ -249,129 +393,14 @@ Ltac simplify_reflection :=
          [| | let r := fresh "r" in
               intro r; destruct r; simpl; reflexivity]) ].
 
-Ltac DSL_term :=
-  repeat match goal with
-    [ H : _ ↝ (?R, _) |- MethodCall_Computes _ _ ?R _ ] =>
-    solve [ econstructor; eassumption
-          | econstructor; [eassumption|higher_order_reflexivity] ]
-  end.
+Ltac compile_term :=
+  repeat (autounfold; simpl);
+  repeat (repeat simplify_reflection; build_computational_spine).
 
-Ltac build_computational_spine :=
-  repeat match goal with
-  | [ |- reflect_ADT_DSL_computation _ _ ] => eexists; intros
-  (* | H : {a' | @?P a'} ↝ _ |- _ => apply Pick_inv in H *)
-  (* | H : Return ?a ↝ _ |- _ => *)
-  (*   apply Return_inv in H; tsubst; try apply CPure *)
-  (* | H : Bind (A := ?A) ?ca ?k ↝ _ |- _ => *)
-  (*   apply Bind_inv in H; *)
-  (*   let a' := fresh "v" in *)
-  (*   let H' := fresh H "'" in *)
-  (*   destruct H as [a' [H H'] ]; *)
-  (*   eapply CJoin *)
-  end;
-  computes_to_inv; tsubst; simpl in *;
-  repeat match goal with
-  | [ H : _ * _ |- _ ] => destruct H
-  | [ H : () |- _ ] => destruct H
-  end.
-
-Lemma lt_0_n : forall n, 0 < n + 1.
-Proof. nomega. Qed.
-
-Ltac wrapup :=
-  first
-  [ eassumption
-  | higher_order_reflexivity
-  | instantiate (1 := eq_sym eq_refl);
-    instantiate (1 := eq_sym eq_refl);
-    reflexivity ].
-
-Definition consDSL w :
-  reflect_ADT_DSL_computation HeapSpec
-    (fun r => r' <- buffer_cons (fst r) (snd r) w; ret (r', ()))%comp.
-Proof.
-  Local Opaque poke.
-  Local Opaque alloc.
-  Local Opaque free.
-  Local Opaque peek.
-  Local Opaque memcpy.
-
-  repeat (autounfold; simpl).
-
-  simplify_reflection.
-    simplify_reflection.
-    { build_computational_spine.
-
-      eapply CJoin.
-      eapply CPure.
-
-      eapply CallComputes
-        with (midx := Fin.FS (Fin.FS (Fin.FS (Fin.FS Fin.F1))))
-             (args := HCons (psBuffer bs + (psOffset bs - 1))
-                            (HCons w HNil)); wrapup.
-    }
-
-  simplify_reflection.
-    simplify_reflection.
-    { build_computational_spine.
-
-      eapply CJoin.
-      eapply CJoin.
-      eapply CPure.
-
-      eapply CallComputes
-        with (midx := Fin.FS (Fin.FS (Fin.FS (Fin.FS Fin.F1))))
-             (args := HCons (psBuffer bs + 0) (HCons w HNil)); wrapup.
-      eapply CallComputes
-        with (midx := Fin.FS (Fin.FS (Fin.FS (Fin.FS (Fin.FS Fin.F1)))))
-             (args := HCons (psBuffer bs) (HCons (psBuffer bs + 1) (HCons (psLength bs) HNil)));
-        wrapup.
-    }
-
-  simplify_reflection.
-    simplify_reflection.
-    { build_computational_spine.
-
-      eapply CJoin.
-      eapply CJoin.
-      eapply CJoin.
-      eapply CJoin.
-      eapply CPure.
-
-      eapply CallCompute2 with (midx := Fin.FS (Fin.FS (Fin.FS (Fin.FS Fin.F1))));
-        wrapup.
-      eapply CallCompute1 with (midx := Fin.FS Fin.F1);
-        wrapup.
-      eapply CallCompute3 with (midx := Fin.FS (Fin.FS (Fin.FS (Fin.FS (Fin.FS Fin.F1)))));
-        wrapup.
-      simpl in *.
-      eapply CallCompute1 with (midx := Fin.F1);
-        wrapup.
-    }
-
-  simplify_reflection.
-    { build_computational_spine.
-
-      eapply CJoin.
-      eapply CJoin.
-      eapply CPure.
-
-      eapply CallCompute2 with (midx := Fin.FS (Fin.FS (Fin.FS (Fin.FS Fin.F1))));
-        wrapup.
-      simpl in *.
-      eapply CallCompute1 with (midx := Fin.F1);
-        wrapup.
-    }
-
-  Local Transparent poke.
-  Local Transparent alloc.
-  Local Transparent free.
-  Local Transparent peek.
-  Local Transparent memcpy.
-Defined.
-
-Definition consDSL' w := Eval simpl in projT1 (consDSL w).
-(* Print consDSL'. *)
+(****************************************************************************
+ * Denote a [ClientDSL] term into a Fiat computation for a particular ADT.
+ * This is strictly the inverse of compilation.
+ ****************************************************************************)
 
 Section Denotation.
 
@@ -386,10 +415,9 @@ Program Instance ADT_Method_Functor :
 Program Instance ADT_Method_Applicative :
   Applicative (fun A : Type => Rep adt -> Comp (Rep adt * A)) := {
   pure := fun _ x r => ret (r, x);
-  ap := fun _ _ mf mx r =>
-            `(r', f) <- mf r;
-            `(r', x) <- mx r';
-            ret (r', f x)
+  ap := fun _ _ mf mx r => `(r', f) <- mf r;
+                           `(r', x) <- mx r';
+                           ret (r', f x)
 }.
 
 Program Instance ADT_Method_Monad :
@@ -399,8 +427,8 @@ Program Instance ADT_Method_Monad :
 
 Import EqNotations.
 
-Definition denote {A : Type} : CallDSL sig A -> Rep adt -> Comp (Rep adt * A) :=
-  foldFree (fun T (c : MethodCall sig T) =>
+Definition denote {A : Type} : ClientDSL sig A -> Rep adt -> Comp (Rep adt * A) :=
+  foldFree (fun T (c : MethodCall T) =>
               match c with
               | Call midx _ _ H1 H2 args k =>
                 fun r =>
@@ -414,7 +442,7 @@ Corollary denote_Pure : forall A (x : A) r,
 Proof. reflexivity. Qed.
 
 Lemma denote_Join :
-  forall A B (k : A -> CallDSL sig B) (h : MethodCall sig A) r,
+  forall A B (k : A -> ClientDSL sig B) (h : MethodCall A) r,
   refineEquiv (denote (Join k h) r)
               (denote (liftF h) r >>= fun p => denote (k (snd p)) (fst p)).
 Proof.
@@ -425,7 +453,7 @@ Proof.
 Qed.
 
 Lemma denote_Free_bind :
-  forall A (x : CallDSL sig A) B (k : A -> CallDSL sig B) r,
+  forall A (x : ClientDSL sig A) B (k : A -> ClientDSL sig B) r,
     refineEquiv (denote (Free_bind k x) r)
                 (denote x r >>= fun p => denote (k (snd p)) (fst p)).
 Proof.
@@ -443,7 +471,7 @@ Proof.
 Qed.
 
 Corollary denote_If :
-  forall b A (t e : CallDSL sig A) r,
+  forall b A (t e : ClientDSL sig A) r,
     refineEquiv (denote (If b Then t Else e) r)
                 (If b Then denote t r Else denote e r).
 Proof. destruct b; simpl; reflexivity. Qed.
@@ -477,6 +505,74 @@ Qed.
 
 End Denotation.
 
+(****************************************************************************
+ * Compile [buffer_cons] into a [ClientDSL] term
+ ****************************************************************************)
+
+Module ByteStringFFI (M : WSfun N_as_DT).
+
+Module Import ByteStringHeap := ByteStringHeap M.
+Module Import FunMaps := FunMaps N_as_DT M.
+
+Import HeapCanonical.
+Import Heap.
+
+Hint Unfold id.
+Hint Unfold bind.
+Hint Unfold Bind2.
+Hint Unfold allocate_buffer.
+Hint Unfold HeapState.find_free_block.
+Hint Unfold make_room_by_growing_buffer.
+Hint Unfold make_room_by_shifting_up.
+Hint Unfold ByteStringHeap.buffer_cons_obligation_2.
+Hint Unfold ByteStringHeap.buffer_cons_obligation_3.
+Hint Unfold poke_at_offset.
+Hint Unfold buffer_cons.
+
+Definition consDSL w :
+  reflect_ADT_DSL_computation HeapSpec
+    (fun r => r' <- buffer_cons (fst r) (snd r) w; ret (r', ()))%comp.
+Proof.
+  Local Opaque poke.
+  Local Opaque alloc.
+  Local Opaque free.
+  Local Opaque peek.
+  Local Opaque memcpy.
+
+  Time compile_term.
+
+  Local Transparent poke.
+  Local Transparent alloc.
+  Local Transparent free.
+  Local Transparent peek.
+  Local Transparent memcpy.
+Defined.
+
+Theorem consDSL_correct : forall (r : Rep HeapSpec) (bs : PS) w,
+  refine (buffer_cons r bs w)
+         (res <- denote HeapSpec (projT1 (consDSL w) bs) r;
+          ret (fst res, fst (snd res))).
+Proof.
+  intros.
+  unfold buffer_cons, consDSL, Bind2; simpl.
+  remember (exist (fun len : Size => 0 < len)
+                  (psLength bs + 1) _) as ev.
+  Time rewrite denote_If, !refineEquiv_If_Then_Else_Bind; simpl.
+  apply refine_If_Then_Else.
+    Time autorewrite with monad laws; reflexivity.
+  Time rewrite denote_If, refineEquiv_If_Then_Else_Bind; simpl.
+  apply refine_If_Then_Else.
+    Time autorewrite with monad laws; reflexivity.
+  Time rewrite denote_If, refineEquiv_If_Then_Else_Bind; simpl.
+  apply refine_If_Then_Else.
+    Time autorewrite with monad laws; reflexivity.
+  Time autorewrite with monad laws; reflexivity.
+Qed.
+
+(****************************************************************************
+ * Denote a [ClientDSL HeapSpec] term into a GHC computation
+ ****************************************************************************)
+
 Axiom IO : Type -> Type.
 
 Axiom fmapIO   : forall {a b : Type}, (a -> b) -> IO a -> IO b.
@@ -498,15 +594,10 @@ Axiom poke    : Ptr Word -> Word -> IO ().
 Axiom memcpy  : Ptr Word -> Ptr Word -> Size -> IO ().
 Axiom memset  : Ptr Word -> Size -> Word -> IO ().
 
-Definition getADTSig {sig : DecoratedADTSig} : ADT sig -> DecoratedADTSig :=
-  fun _ => sig.
-
-Definition ghcDenote {A : Type} : CallDSL (getADTSig HeapSpec) A -> A.
+Definition ghcDenote {A : Type} : ClientDSL (getADTSig HeapSpec) (IO A) -> IO A.
 Proof.
   intros.
-  apply (fmap returnIO) in X.
   eapply (iter _) in X.
-  apply unsafeDupablePerformIO in X.
   exact X.
   Unshelve.
   clear X.
@@ -514,25 +605,25 @@ Proof.
   subst.
   simpl in midx.
   dependent destruction midx; simpl in *.
-    inv e0. inv h. inv X0.
+    inv e0. inv h.
     exact (bindIO (malloc (` X)) i).
   dependent destruction midx; simpl in *.
-    inv e0. inv h. inv X0.
+    inv e0. inv h.
     exact (bindIO (free X) i).
   dependent destruction midx; simpl in *.
-    inv e0. inv h. inv X0. inv X2.
+    inv e0. inv h. inv X0.
     exact (bindIO (realloc X (` X1)) i).
   dependent destruction midx; simpl in *.
-    inv e0. inv h. inv X0.
+    inv e0. inv h.
     exact (bindIO (peek X) i).
   dependent destruction midx; simpl in *.
-    inv e0. inv h. inv X0. inv X2.
+    inv e0. inv h. inv X0.
     exact (bindIO (poke X X1) i).
   dependent destruction midx; simpl in *.
-    inv e0. inv h. inv X0. inv X2. inv X3.
+    inv e0. inv h. inv X0. inv X2.
     exact (bindIO (memcpy X X1 X0) i).
   dependent destruction midx; simpl in *.
-    inv e0. inv h. inv X0. inv X2. inv X3.
+    inv e0. inv h. inv X0. inv X2.
     exact (bindIO (memset X X1 X0) i).
   inversion midx.
 Defined.
@@ -549,62 +640,46 @@ Corollary iter_If `{Functor f} : forall A (phi : f A -> A) b t e,
   iter phi (If b Then t Else e) = If b Then iter phi t Else iter phi e.
 Proof. destruct b; reflexivity. Qed.
 
+Corollary ghcDenote_If : forall A b (t e : ClientDSL (getADTSig HeapSpec) (IO A)),
+  ghcDenote (If b Then t Else e) = If b Then ghcDenote t Else ghcDenote e.
+Proof. destruct b; reflexivity. Qed.
+
 Lemma ghcConsDSL :
   { f : PS -> Word -> PS
-  & forall bs w, f bs w = ghcDenote (fst <$> projT1 (consDSL w) bs) }.
+  & forall bs w,
+      f bs w = unsafeDupablePerformIO
+                 (ghcDenote ((returnIO \o fst) <$> projT1 (consDSL w) bs)) }.
 Proof.
-  eexists.
-  intros.
-  unfold consDSL, ghcDenote, compose, comp.
+  eexists; intros.
   symmetry.
   simpl projT1.
-  do 6 rewrite fmap_If.
+  unfold comp.
+  rewrite !fmap_If.
+  etransitivity.
+    do 3 setoid_rewrite ghcDenote_If.
+    reflexivity.
   simpl.
-  do 3 setoid_rewrite iter_If.
-  simpl.
-  unfold If_Then_Else, compose, comp; simpl.
-  unfold solution_left, eq_rect_r, eq_rect.
-  simpl.
+  do 4 (unfold compose, comp; simpl).
+  unfold ghcDenote; simpl.
+  unfold solution_left.
+  unfold eq_rect_r, eq_rect; simpl.
   unfold simplification_heq.
-  unfold solution_right, eq_rect_r, eq_rect.
-  simpl.
-  unfold block.
-  simpl.
-  unfold eq_sym.
-Admitted.
+  unfold solution_right.
+  unfold eq_rect_r, eq_rect; simpl.
+  repeat (rewrite JMeq_eq_refl; unfold compose, comp; simpl).
+  rewrite !bindIO_returnIO.
+  higher_order_reflexivity.
+Defined.
 
 Definition ghcConsDSL' := Eval simpl in projT1 ghcConsDSL.
-(* Print ghcConsDSL'. *)
-
-Theorem consDSL_correct : forall (r : Rep HeapSpec) (bs : PS) w,
-  refine (buffer_cons r bs w)
-         (res <- denote HeapSpec (projT1 (consDSL w) bs) r;
-          ret (fst res, fst (snd res))).
-Proof.
-  intros.
-  destruct r.
-  unfold buffer_cons, consDSL; simpl.
-  repeat rewrite denote_Free_bind; simpl.
-  rewrite denote_If; simpl.
-  unfold Bind2.
-  do 4 rewrite refineEquiv_If_Then_Else_Bind.
-  apply refine_If_Then_Else.
-    autorewrite with monad laws; reflexivity.
-  rewrite denote_If; simpl.
-  rewrite refineEquiv_If_Then_Else_Bind.
-  apply refine_If_Then_Else.
-    autorewrite with monad laws; reflexivity.
-  rewrite denote_If; simpl.
-  rewrite refineEquiv_If_Then_Else_Bind.
-  apply refine_If_Then_Else.
-    autorewrite with monad laws; reflexivity.
-  autorewrite with monad laws; reflexivity.
-Qed.
+Print ghcConsDSL'.
 
 End ByteStringFFI.
 
-(** This is the code we intend to approximate with the FFI refined version of
-    ByteString:
+(****************************************************************************
+
+This is the code we intend to approximate with the FFI refined version of
+ByteString:
 
   import Data.Word8
   import GHC.ForeignPtr
@@ -651,4 +726,5 @@ End ByteStringFFI.
       | otherwise = Just (accursedUnutterablePerformIO $ withForeignPtr x
                                                        $ \p -> peekByteOff p s,
                           PS x (s+1) (l-1))
-*)
+
+****************************************************************************)
