lib/HList.v
@@ -1,0 +1,47 @@
+Require Import
+  Coq.Lists.List.
+
+Generalizable All Variables.
+
+Import ListNotations.
+
+(****************************************************************************
+ * hlist: Type heterogeneous list indexed by a list.
+ ****************************************************************************)
+
+Inductive hlist : list Type -> Type :=
+  | HNil : hlist []
+  | HCons : forall t ts, t -> hlist ts -> hlist (t :: ts).
+
+Arguments HNil : default implicits.
+Arguments HCons : default implicits.
+
+Lemma cons_head_eq : forall A (x0 : A) x1 y0 y1,
+  x0 :: y0 = x1 :: y1 -> x0 = x1.
+Proof.
+  intros.
+  inversion H.
+  intuition.
+Defined.
+
+Lemma cons_tail_eq : forall A (x0 : A) x1 y0 y1,
+  x0 :: y0 = x1 :: y1 -> y0 = y1.
+Proof.
+  intros.
+  inversion H.
+  intuition.
+Defined.
+
+Import EqNotations.
+
+Program Definition hlist_head `(l : hlist (t :: ts)) : t :=
+  match l in hlist d return d = t :: ts -> t with
+  | HNil => fun _ => False_rect _ _
+  | HCons x _ => fun H => rew (cons_head_eq _ _ _ _ _ H) in x
+  end eq_refl.
+
+Program Definition hlist_tail `(l : hlist (t :: ts)) : hlist ts :=
+  match l in hlist d return d = t :: ts -> hlist ts with
+  | HNil => fun _ => False_rect _ _
+  | HCons _ xs => fun H => rew (cons_tail_eq _ _ _ _ _ H) in xs
+  end eq_refl.
