src/ByteStringCanon.v
@@ -37,41 +37,32 @@ Variable heap_AbsR : Heap_AbsR heap heap'.
    mean going directly to the metal (but would require replicating much of the
    proof work that is done in HeapFMap.v). *)
 
-Record ByteString_Heap_AbsR or nr := {
-  heap_match   : Heap_AbsR (psHeap or) (psHeap nr);
-  buffer_match : psBuffer or = psBuffer nr;
-  buflen_match : psBufLen or = psBufLen nr;
-  offset_match : psOffset or = psOffset nr;
-  length_match : psLength or = psLength nr
-}.
-
 Lemma refine_ByteString_Heap_AbsR :
   forall heap_resvs heap_bytes buffer buflen offset length B (k : _ -> Comp B),
     refine
-      (r_n' <- { r_n0 : PS cHeapRep
-               | ByteString_Heap_AbsR
-                   {| psHeap := {| resvs := heap_resvs
-                                 ; bytes := heap_bytes |}
-                    ; psBuffer := buffer
-                    ; psBufLen := buflen
-                    ; psOffset := offset
-                    ; psLength := length |} r_n0 };
+      (r_n' <- { r_n0 : cHeapRep * PS
+               | Heap_AbsR {| resvs := heap_resvs
+                            ; bytes := heap_bytes |} (fst r_n0) /\
+                 {| psBuffer := buffer
+                  ; psBufLen := buflen
+                  ; psOffset := offset
+                  ; psLength := length |} = snd r_n0 };
        k r_n')
       (resvs' <- {resvs' : M.t Size | M.Equal heap_resvs resvs'};
        bytes' <- {bytes' : M.t Word | M.Equal heap_bytes bytes'};
        brk'   <- {brk'   : N
                  | P.for_all (fun addr sz => addr + sz <=? brk') resvs' };
-       k {| psHeap   := (brk', {| resvs := resvs'; bytes := bytes' |})
-          ; psBuffer := buffer
-          ; psBufLen := buflen
-          ; psOffset := offset
-          ; psLength := length |}).
+       k ((brk', {| resvs := resvs'; bytes := bytes' |}),
+          {| psBuffer := buffer
+           ; psBufLen := buflen
+           ; psOffset := offset
+           ; psLength := length |})).
 Proof.
   intros; intros ??.
   destruct_computations.
   revert H2.
-  remember (makePS _ _ _ _ _) as P; intros.
-  refine pick val P.
+  remember (makePS _ _ _ _) as P; intros.
+  refine pick val ((x1, {| resvs := x; bytes := x0 |}), P).
     apply computes_to_refine.
     simplify with monad laws.
     apply refine_computes_to.
@@ -82,14 +73,12 @@ Qed.
 
 Ltac apply_ByteString_Heap_AbsR :=
   match goal with
-    | [ H : ByteString_Heap_AbsR ?O ?N |- _ ] =>
+    | [ H : Heap_AbsR (fst ?O) (fst ?N) /\ snd ?X = snd ?Y |- _ ] =>
       destruct H as
-          [ [ resvs_match0 [ bytes_match0 for_all_matches0 ] ]
-            buffer_match0 buflen_match0 offset_match0 length_match0 ],
-          O as [ [ resvs_o bytes_o ]
-                 psBuffer0 psBufLen0 psOffset0 psLength0 ];
+          [ [ resvs_match0 [ bytes_match0 for_all_matches0 ] ] match0 ],
+          O as [ [ resvs_o bytes_o ] ps_o ];
       simpl in *;
-      rewrite ?buffer_match0, ?buflen_match0, ?offset_match0, ?length_match0
+      rewrite ?match0
   end.
 
 Tactic Notation "refine" "using" "ByteString_Heap_AbsR" :=
@@ -104,7 +93,8 @@ Tactic Notation "refine" "using" "ByteString_Heap_AbsR" :=
         match goal with
         | [ |- refine (x <- ret _; _) _ ] =>
           simplify with monad laws; simpl
-        | [ |- refine (x <- { X : PS cHeapRep | ByteString_Heap_AbsR _ X }; _) _ ] =>
+        | [ |- refine (x <- { X : cHeapRep * PS
+                            | Heap_AbsR _ (fst X) /\ _ = snd X }; _) _ ] =>
           rewrite refine_ByteString_Heap_AbsR
         | [ |- refine (If ?B Then ?T Else ?E) _ ] =>
           apply refine_If_Then_Else
@@ -128,16 +118,16 @@ Theorem ByteStringCanonical : FullySharpened (projT1 (ByteStringHeap heap)).
 Proof.
   start sharpening ADT.
 
-  hone representation using ByteString_Heap_AbsR.
+  hone representation using
+       (fun or nr => Heap_AbsR (fst or) (fst nr) /\ snd or = snd nr).
 
   refine method ByteString.emptyS.
   {
     simplify with monad laws.
-    refine pick val {| psHeap   := heap'
-                     ; psBuffer := 0
-                     ; psBufLen := 0
-                     ; psOffset := 0
-                     ; psLength := 0 |}.
+    refine pick val (heap', {| psBuffer := 0
+                             ; psBufLen := 0
+                             ; psOffset := 0
+                             ; psLength := 0 |}).
       finish honing.
     firstorder.
   }
@@ -147,13 +137,13 @@ Proof.
     apply_ByteString_Heap_AbsR.
     fracture H; unfold find_free_block;
     refine using ByteString_Heap_AbsR;
-    refine pick val (fst (psHeap r_n)); eauto;
+    refine pick val (fst (fst r_n)); eauto;
     try simplify with monad laws;
     try finish honing;
     refine using ByteString_Heap_AbsR.
 
-    - refine pick val (fst (psHeap r_n) +
-                       (psLength r_n + alloc_quantum)); eauto.
+    - refine pick val (fst (fst r_n) +
+                       (psLength (snd r_n) + alloc_quantum)); eauto.
         simplify with monad laws.
         finish honing.
 
@@ -170,7 +160,7 @@ Proof.
       eapply for_all_impl; eauto;
       relational; nomega.
 
-    - refine pick val (fst (psHeap r_n) + alloc_quantum); eauto.
+    - refine pick val (fst (fst r_n) + alloc_quantum); eauto.
         simplify with monad laws.
         finish honing.
 
@@ -194,13 +184,13 @@ Proof.
     fracture H;
     refine using ByteString_Heap_AbsR.
 
-    - refine pick val (Ifopt M.find (psBuffer r_n + psOffset r_n)
-                                    (bytes (snd (psHeap r_n))) as v
+    - refine pick val (Ifopt M.find (psBuffer (snd r_n) + psOffset (snd r_n))
+                                    (bytes (snd (fst r_n))) as v
                        Then v
                        Else Zero).
         simplify with monad laws.
         refine using ByteString_Heap_AbsR.
-        refine pick val (fst (psHeap r_n)); eauto.
+        refine pick val (fst (fst r_n)); eauto.
         simplify with monad laws.
         finish honing.
 
@@ -212,9 +202,11 @@ Proof.
       apply F.find_mapsto_iff in H.
       congruence.
 
-    - refine pick val (fst (psHeap r_n)); eauto.
-      simplify with monad laws.
-      finish honing.
+    - refine pick val r_n; eauto.
+        simplify with monad laws.
+        finish honing.
+      split; trivial.
+      constructor; auto.
   }
 
   (** Apply some common functional optimizations, such as common subexpression
@@ -236,11 +228,11 @@ Proof.
     simplify with monad laws.
     rewrite !If_Then_Else_fst, !If_Then_Else_snd; simpl.
 
-    replace (If 0 <? psOffset r_o
+    replace (If 0 <? psOffset (snd r_o)
              Then ()
-             Else (If psLength r_o + 1 <=? psBufLen r_o
+             Else (If psLength (snd r_o) + 1 <=? psBufLen (snd r_o)
                    Then ()
-                   Else (If 0 <? psBufLen r_o
+                   Else (If 0 <? psBufLen (snd r_o)
                          Then ()
                          Else ()))) with ().
       subst; finish honing.
